through April 22, 2020

lists.dfy
@@ -58,6 +58,11 @@ ghost method testGetElementAtIndex() {
 	assert getElementAtIndex(Cons(2, Cons(1, Nil)), 0) == 2;
 }
 
+function method listToSeq<A>(list: List<A>): seq<A>
+{
+	if (list.Nil?) then [] else [list.head] + listToSeq(list.tail)
+}
+
 // Cons(1, Cons(2, Cons(3, Nil))): [1, 2, 3]
 // take([1, 2, 3], 0) == []
 // take([1, 2, 3], 1) == [1]
@@ -70,5 +75,13 @@ ghost method testGetElementAtIndex() {
 //
 function method take<A>(list: List<A>, amount: int): List<A>
 	requires 0 <= amount <= length(list);
+	ensures length(take(list, amount)) == amount;
+	ensures forall i :: 0 <= i < amount ==>
+		getElementAtIndex(list, i) == getElementAtIndex(take(list, amount), i);
+  //ensures listToSeq(list)[..amount - 1] == listToSeq(take(list, amount));
+	// 1.) define the body of take
+	//     - Need recursion
+	// 2.) postconditions
 {
+	if (amount == 0) then Nil else Cons(list.head, take(list.tail, amount - 1))
 }
